Fixed typed issues

Examples/memcpy_lo_memcpy_armv8_proof.v
@@ -44,77 +44,37 @@ Definition filled m dest src len :=
   N.recursion m (fun i m' => m'[Ⓑ dest + i := m Ⓑ[src + i]]) len.
   
 Section Invariants.
-    
-    Variable sp : N          (* initial stack pointer *).
-    Variable mem : memory    (* initial memory state *).
-    Variable raddr : N       (* return address (R_X30) *).
+  Variable mem : memory    (* initial memory state *).
 
-    (* Variable dest : N        (* memcpy: 1st pointer arg (R_X0), destination address *).
-    Variable src : N        (* memcpy: 2nd pointer arg (R_X1), source address *).
-    Variable len : N        (* memcpy: 2nd pointer arg (R_X2), byte count *). *)
+  Variable dest : N        (* memcpy: 1st pointer arg (R_X0), destination address *).
+  Variable src : N        (* memcpy: 2nd pointer arg (R_X1), source address *).
+  Variable len : N        (* memcpy: 2nd pointer arg (R_X2), byte count *).
   
   (* Registers state after copying k bytes *)
-  Definition memcpy_regs (s : store) src dest len k :=
+  Definition memcpy_regs (s : store) k :=
     s V_MEM64 = filled mem dest src k /\
-    s R_X0 = src /\
-    s R_X1 = dest /\
+    s R_X0 = dest /\
+    s R_X1 = src /\
     s R_X2 = (len - k).
 
   (* Loop invariant: k bytes copied so far *)
-  Definition memcpy_inv (s : store) dest src len (k : N)  :=
+  Definition memcpy_inv (s : store) (k : N)  :=
     k <= len /\
-    memcpy_regs s dest src len k.
+    memcpy_regs s k.
 
-  Definition bounds_safe (dest src len : N) :=
+  Definition bounds_safe :=
     dest + len < 2^64 /\ src + len < 2^64 /\ len < 2^64.
 
-(* Remove?
-  Definition align_inv dest (s : store) :=
-    s R_X14 = dest mod 16 /\
-    s R_X3 = dest - (dest mod 16). *)
-(* 
-  (* Postcondition: all bytes copied correctly *)
-  Definition postcondition dest src len (s : store) :=
-    s R_X0 = dest /\
-    s V_MEM64 = filled mem dest src len. *)
-(* 
-Definition memcpy_invset (t : trace) :=
-  match t with
-  | (Addr a, s) :: _ =>
-      if a =? 0x100000 then Some (
-        s R_X0 = dest /\ 
-        s R_X1 = src /\ 
-        s R_X2 = len /\ 
-        s R_X30 = raddr /\ 
-        dest + len < 2 ^ 64 /\ 
-        src + len < 2 ^ 64
-        )
-(*
-      (* 16 byte copy *) else if a =? 0x100020 then Some (16 <= len /\ s R_X0 = dest /\ s R_X1 = src /\ s R_X2 = len /\ s R_X4 = src + len /\ s R_X5 = dest + len) 
-      (* Small byte copy *) else if a =? 1048628 then Some (∃ k, memcpy_inv s k) *)
-      else if a =? 0x100130 then Some (exists k : N,
-      k <= len /\
-      s V_MEM64 = filled mem dest src k /\
-      s R_X0 = dest /\
-      s R_X1 = src /\
-      s R_X2 = len - k /\
-      s R_X30 = raddr
-      )
-
-      else None
-  | _ => None
-  end. *)
-
-Definition memcpy_invset' mem dest src len (k : N) (t : trace) : option Prop :=
+Definition memcpy_invset' (t : trace) : option Prop :=
   match t with
   | (Addr a, s) :: _ =>
       match a with
 
       (* Entry point *)
-      | 0x100000 => Some (memcpy_regs s dest src len 0)
+      | 0x100000 => Some (memcpy_regs s 0)
 
       (* Loop 1 (1-byte writes to word boundary) *)
-      | 0x100130 => Some (memcpy_regs s dest src len k /\ s V_MEM64 = filled mem dest src k)
+      | 0x100130 => Some (exists mem k, memcpy_regs s k /\ s V_MEM64 = filled mem dest src k)
 
       (* post-condition: *)
       | 0x100188 
@@ -123,7 +83,7 @@ Definition memcpy_invset' mem dest src len (k : N) (t : trace) : option Prop :=
       | 0x100064 
       | 0x100048 
       | 0x100030 
-      | 0x1000b8 => Some (memcpy_regs s dest src len len /\ s V_MEM64 = filled mem dest src len)
+      | 0x1000b8 => Some (exists mem, memcpy_regs s len /\ s V_MEM64 = filled mem dest src len)
 
       | _ => None
       end
@@ -132,8 +92,6 @@ Definition memcpy_invset' mem dest src len (k : N) (t : trace) : option Prop :=
 
 
 End Invariants.
-    
-
 
 
 Lemma filled0: ∀ m p c, filled m p c 0 = m.
@@ -248,7 +206,7 @@ Theorem memcpy_partial_correctness:
     (DIST: (dest + len < src) \/ (src + len < dest))
     (K_lim: 0 <= k <= len),
     satisfies_all memcpy_lo_memcpy_armv8
-    (fun t0 => memcpy_invset' mem (s R_X0) dest src len k t0)
+    (memcpy_invset' mem dest src len)
     program_exit
     ((x', s')::t).
 Proof.
@@ -259,31 +217,18 @@ Proof.
   (* Base case: entry invariant *)
   simpl. rewrite ENTRY. step.
   repeat split; try assumption.
-  intros. destruct_inv 64 PRE.
+  intros. 
+  
+  destruct_inv 64 PRE.
   erewrite startof_prefix in ENTRY; try eassumption. 
   destruct PRE as [MEM' [R0' [R1' R2']]].
-  step. step. step. step. step. step. step.
-  step. step. step. step. step. rewrite filled0 in MEM'. 
+  repeat step. rewrite filled0 in MEM'. 
   erewrite filled0. repeat eexists; psimpl; try (eassumption || reflexivity).
   
   
   
-assert (LEN64 := models_var R_X2 MDL). rewrite R2 in LEN64. unfold arm8typctx in LEN64.
-auto. psimpl.
-
-(* length = 0, exit point *)
-try eassumption. psimpl in K_lim.
-
-erewrite MEM. induction k as [|k'] using N.peano_ind; psimpl; try (eassumption || reflexivity).
-unfold filled. induction N.recursion using N.peano_ind.
-induction N.recursion eqn: Hr using N.peano_ind. reflexivity.
-(* Inductive case *)
-
-  
-  apply memcpy_welltyped. 
-  eapply models_at_invariant; try eassumption. apply memcpy_welltyped. intro MDL1.
-  clear - PRE MDL1 LEN64.
- (* rename t1 into t.*) rename s1 into s1'. rename MDL1 into MDL.
+  assert (LEN64 := models_var R_X2 MDL). rewrite R2 in LEN64. unfold arm8typctx in LEN64.
+  auto. psimpl.
   
 Admitted.
  
